execution/theories/ProgramError.v
@@ -1,0 +1,33 @@
+From Coq Require Import String.
+From ConCert.Execution Require Import Monads.
+From ConCert.Execution Require Import ResultMonad.
+
+Inductive ProgramError :=
+| Custom {Error : Type} (e : Error)
+| InvalidArgument
+| InvalidInstructionData
+| InvalidAccountData
+| AccountDataTooSmall
+| InsufficientFunds
+| IncorrectProgramId
+| MissingRequiredSignature
+| AccountAlreadyInitialized
+| UninitializedAccount
+| NotEnoughAccountKeys
+| AccountBorrowFailed
+| MaxSeedLengthExceeded
+| InvalidSeeds
+| BorshIoError (s : string)
+| AccountNotRentExempt
+| UnsupportedSysvar
+| IllegalOwner
+| MaxAccountsDataSizeExceeded
+| InvalidRealloc.
+
+Global Instance Monad_result_error : Monad (fun T => result T ProgramError) :=
+  {| ret _ t := Ok t;
+     bind _ _ mt f :=
+     match mt with
+     | Ok t => f t
+     | Err e => Err e
+     end |}.
